\[\text{grad}\Phi=\vec{a_x}\frac{\partial\Phi}{\partial x}+\vec{a_y}\frac{\partial\Phi}{\partial y}+\vec{a_z}\frac{\partial\Phi}{\partial z}=\nabla\Phi\]

> Nabla Symbol ($\nabla$): $\nabla=\vec{a_x}\frac{\partial}{\partial x}+\vec{a_y}\frac{\partial}{\partial y}+\vec{a_z}\frac{\partial}{\partial z}$.

\[\nabla\Phi=\vec{a_x}\frac{\partial\Phi}{\partial x}+\vec{a_y}\frac{\partial\Phi}{\partial y}+\vec{a_z}\frac{\partial\Phi}{\partial z}\]

\[\nabla\Phi=\vec{a_\rho}\frac{\partial\Phi}{\partial\rho}+\vec{a_\varphi}\frac{\partial\Phi}{\rho\partial\varphi}+\vec{a_z}\frac{\partial\Phi}{\partial z}\]

\[\nabla\Phi=\vec{a_r}\frac{\partial\Phi}{\partial r}+\vec{a_\theta}\frac{\partial\Phi}{r\partial\theta}+\vec{a_\varphi}\frac{\partial\Phi}{r\sin\theta\partial\varphi}\]

\[\nabla C=\vec{0}\]
\[\nabla(Cu)=C\nabla u\]
\[\nabla(u\mp v)=\nabla u\mp\nabla v\]
\[\nabla(uv)=u\nabla v+v\nabla u\]
\[\nabla f(u)=f'(u)\nabla u\]

